nola/iris/inv_deriv.v
@@ -4,38 +4,41 @@ From nola.iris Require Export util deriv inv.
 From iris.proofmode Require Import proofmode.
 Import PintpNotation DerivNotation.
 
-Section inv_deriv.
-  Context `{!inv'GS PROP Σ, !invGS_gen hlc Σ}.
-
-  (** Accessor *)
-  Definition inv_acsr' intp N P : iProp Σ :=
-    ∀ E, ⌜↑N ⊆ E⌝ → |=[inv_wsat intp]{E,E∖↑N}=>
-      P ∗ (P =[inv_wsat intp]{E∖↑N,E}=∗ True).
-
-  (** Derivability data for [inv] *)
-  Class DerivInv (JUDG : judg (iProp Σ)) := DERIV_INV {
-    deriv_inv_intp ::
-      Pintp (deriv JUDG (iProp Σ)) (PROP $o iProp Σ) (iProp Σ);
-    deriv_inv_ne {δ} :: NonExpansive (deriv_inv_intp δ);
-    deriv_inv_acsr : namespace → PROP $o iProp Σ → JUDG;
-    deriv_inv_acsr_intp {δ N P} :
-      ⟦ deriv_inv_acsr N P ⟧(δ) ≡ inv_acsr' ⟦⟧(δ) N ⟦ P ⟧(δ);
-  }.
-End inv_deriv.
 (** Notation *)
-Notation inv_ascr δ N P := (inv_acsr' ⟦⟧(δ) N P).
 Notation inv_wsatd δ := (inv_wsat ⟦⟧(δ)).
 
+(** Derivability pre-data for [inv] *)
+Class InvPreDeriv PRO JUD := inv_jacsr : namespace → PRO → JUD.
+Hint Mode InvPreDeriv ! - : typeclass_instances.
+
 Section inv_deriv.
-  Context `{!inv'GS PROP Σ, !invGS_gen hlc Σ, !DerivInv JUDG}.
-  Implicit Type P Q : PROP $o iProp Σ.
+  Context `{!InvPreDeriv PRO JUD} {Σ : gFunctors}.
 
   (** [inv']: Relaxed invariant *)
-  Definition inv' δ N P : iProp Σ := □ ⸨ deriv_inv_acsr N P ⸩(δ).
+  Definition inv' δ N (P : PRO) : iProp Σ := □ ⸨ inv_jacsr N P ⸩(δ).
 
   (** [inv'] is persistent *)
   Fact inv'_persistent {δ N P} : Persistent (inv' δ N P).
   Proof. exact _. Qed.
+End inv_deriv.
+
+Section inv_deriv.
+  Context `{!inv'GS PROP Σ, !invGS_gen hlc Σ}.
+  Implicit Type P Q PQ : PROP $o iProp Σ.
+
+  (** Accessor *)
+  Definition inv_acsr intp N Pi : iProp Σ :=
+    ∀ E, ⌜↑N ⊆ E⌝ → |=[inv_wsat intp]{E,E∖↑N}=>
+      Pi ∗ (Pi =[inv_wsat intp]{E∖↑N,E}=∗ True).
+
+  Context `{!InvPreDeriv (PROP $o iProp Σ) (JUDG : judg (iProp Σ)),
+    !Dintp JUDG (PROP $o iProp Σ) (iProp Σ)}.
+
+  (** Derivability data for [inv] *)
+  Class InvDeriv :=
+    inv_jacsr_intp : ∀{δ N P}, ⟦ inv_jacsr N P ⟧(δ) ≡ inv_acsr ⟦⟧(δ) N ⟦ P ⟧(δ).
+
+  Context `{!InvDeriv}.
 
   (** Access [inv'] *)
   Lemma inv'_acc {N P E} : ↑N ⊆ E →
@@ -43,7 +46,7 @@ Section inv_deriv.
       ⟦ P ⟧(der) ∗ (⟦ P ⟧(der) =[inv_wsatd der]{E∖↑N,E}=∗ True).
   Proof.
     iIntros (?) "accP". iDestruct (der_sound with "accP") as "accP".
-    rewrite deriv_inv_acsr_intp. by iApply "accP".
+    rewrite inv_jacsr_intp. by iApply "accP".
   Qed.
 
   Context `{!Deriv (JUDG:=JUDG) ih δ}.
@@ -52,7 +55,8 @@ Section inv_deriv.
   Lemma inv_tok_inv' {N P} : inv_tok N P ⊢ inv' δ N P.
   Proof.
     iIntros "#i !>". iApply Deriv_intro. iIntros (? _ _).
-    rewrite deriv_inv_acsr_intp. iIntros (??). by iApply (inv_tok_acc with "i").
+    rewrite inv_jacsr_intp. iIntros (??).
+    by iApply (inv_tok_acc (intp:=⟦⟧(_)) with "i").
   Qed.
 
   (** Allocate [inv'] *)
@@ -68,7 +72,7 @@ Section inv_deriv.
       inv' δ N Q -∗ inv' δ N P.
   Proof.
     iIntros "#QPQ #accQ !>". iApply Deriv_byintp. iIntros (? _ _) "#→ _".
-    iDestruct ("→" with "accQ") as "{accQ}accQ". rewrite !deriv_inv_acsr_intp.
+    iDestruct ("→" with "accQ") as "{accQ}accQ". rewrite !inv_jacsr_intp.
     iIntros (? NE). iMod ("accQ" $! _ NE) as "[Q cl]".
     iMod (fupd_mask_subseteq ∅) as "→E∖N"; [set_solver|].
     iMod ("QPQ" with "Q") as "($& PQ)". iMod "→E∖N" as "_". iIntros "!> P".
@@ -96,7 +100,7 @@ Section inv_deriv.
     inv' δ N1 P -∗ inv' δ N2 Q -∗ inv' δ N PQ.
   Proof.
     iIntros (?? eq) "#i #i' !>". iApply (Deriv_map2 with "[] i i'").
-    iIntros (? _ _) "{i}i {i'}i'". rewrite !deriv_inv_acsr_intp. iIntros (??).
+    iIntros (? _ _) "{i}i {i'}i'". rewrite !inv_jacsr_intp. iIntros (??).
     rewrite eq. iMod ("i" with "[%]") as "[$ P→]"; [set_solver|].
     iMod ("i'" with "[%]") as "[$ Q→]"; [set_solver|].
     iApply fupdw_mask_intro; [set_solver|]. iIntros "cl [P Q]".
